src/TV/symexe_sound.v
@@ -1,6 +1,7 @@
 Add LoadPath "../Vellvm/ott".
 Add LoadPath "../Vellvm/monads".
 Add LoadPath "../Vellvm/compcert".
+Add LoadPath "../Vellvm/GraphBasics".
 Add LoadPath "../Vellvm".
 Add LoadPath "../../../theory/metatheory_8.3".
 Require Import syntax.
@@ -65,16 +66,18 @@ Lemma value2Sterm_denote__imply__genericvalues : forall l0 TD lc0 Mem0 smap1 lc
   uniq smap1 ->
   smap_denotes_gvmap TD lc0 gl Mem0 smap1 lc ->
   sterms_denote_genericvalues TD lc0 gl Mem0 
-    (make_list_sterm (map_list_value (value2Sterm smap1) l0)) gvs0 ->
+    (make_list_sterm 
+      (map_list_sz_value 
+        (fun sz' v' => (sz', value2Sterm smap1 v')) l0)) gvs0 ->
   @values2GVs DGVs TD l0 lc gl = Some gvs0.
 Proof.
   induction l0; intros; simpl in *.
     inversion H1; subst; auto.
 
     inversion H1; subst.
-    apply value2Sterm_denotes__implies__genericvalue with (lc:=lc)(gl:=gl) in H10
+    apply value2Sterm_denotes__implies__genericvalue with (lc:=lc)(gl:=gl) in H11
       ; auto.
-    rewrite H10.
+    rewrite H11.
     erewrite IHl0; eauto.
 Qed.
 
@@ -561,8 +564,10 @@ Proof.
 
     right. 
     exists (sterm_gep i1 t
-                     (value2Sterm st.(STerms) v)
-                     (make_list_sterm (map_list_value (value2Sterm st.(STerms)) l0))). auto.
+             (value2Sterm st.(STerms) v)
+             (make_list_sterm 
+               (map_list_sz_value 
+                 (fun sz' v' => (sz', value2Sterm st.(STerms) v')) l0))). auto.
 
     right. 
     exists (sterm_trunc t t0
@@ -2389,6 +2394,6 @@ Qed.
 (*
 *** Local Variables: ***
 *** coq-prog-name: "coqtop" ***
-*** coq-prog-args: ("-emacs-U" "-I" "~/SVN/sol/vol/src/Vellvm/monads" "-I" "~/SVN/sol/vol/src/Vellvm/ott" "-I" "~/SVN/sol/vol/src/Vellvm/compcert" "-I" "~/SVN/sol/theory/metatheory_8.3") ***
+*** coq-prog-args: ("-emacs-U" "-I" "~/SVN/sol/vol/src/Vellvm/monads" "-I" "~/SVN/sol/vol/src/Vellvm/ott" "-I" "~/SVN/sol/vol/src/Vellvm/compcert" "-I" "~/SVN/sol/theory/metatheory_8.3" "-impredicative-set") ***
 *** End: ***
  *)
